Fixed bug in preprocessing and made new tests

QuerySMT/smallTests.lean
@@ -33,11 +33,38 @@ set_option pp.explicit true in
 #check -Int.ofNat 1 * 5
 -- this one shouldn't be bad
 
+inductive myType2 (t : Type)
+| const3 : t → myType2 t
+| const4 : t → myType2 t
+
+open myType2
+
+example (t : Type) (x : myType2 t) : ∃ y : t, x = const3 y ∨ x = const4 y := by
+  querySMT
+
+set_option querySMT.filterRedundancies true in
+example (t : Type) (x : myType2 t) : ∃ y : t, x = const3 y ∨ x = const4 y := by
+  apply @Classical.byContradiction
+  intro negGoal
+  obtain ⟨_const3__sel0, _const3__sel0Fact⟩ :
+    ∃ (_const3__sel0 : myType2 t → t), ∀ (arg0 : t), _const3__sel0 (const3 arg0) = arg0 :=
+    by
+    apply Exists.intro (rec (motive := fun (_ : myType2 t) => t) (fun (arg0 : t) => arg0) fun (arg0 : t) => sorry)
+    intros
+    rfl
+  obtain ⟨_const4__sel0, _const4__sel0Fact⟩ :
+    ∃ (_const4__sel0 : myType2 t → t), ∀ (arg0 : t), _const4__sel0 (const4 arg0) = arg0 :=
+    by
+    apply Exists.intro (rec (motive := fun (_ : myType2 t) => t) (fun (arg0 : t) => sorry) fun (arg0 : t) => arg0)
+    intros
+    rfl
+  duper [negGoal, _const3__sel0Fact, _const4__sel0Fact] []
+
 set_option pp.explicit true in
 example (x y z : Int) : x ≤ y → y ≤ z → x ≤ z := by
   querySMT
 
-example (f : Int → Int) (h1 : ∀ x y, f x = f y → x = y)
+example (f : Int → Int) (bv1 : ∀ x y, f x = f y → x = y)
 (h2 : ∃ x, ∀ y, f x ≤ f y) : ∃ x, ∀ y, x ≠ y → f x < f y := by
   querySMT
   -- WITH REDUNDANCIES REMOVED, small problem, it needed an extra lemma
@@ -65,7 +92,7 @@ example (f : Int → Int) (h1 : ∀ x y, f x = f y → x = y)
     (¬f sk0 + -Int.ofNat 1 * f (sk1 sk0) ≥ Int.ofNat 0 ∨ f sk0 = f (sk1 sk0)) ∨
       f sk0 + -Int.ofNat 1 * f (sk1 sk0) ≥ Int.ofNat 1 :=
     by grind
-  duper [h1, h2, negGoal, smtLemma0, smtLemma1, smtLemma3] []
+  duper [h1, smtLemma0, smtLemma1, smtLemma2, smtLemma3] []
 
 example (f : Int → Int) (h1 : ∀ x y, f x = f y → x = y)
   (h2 : ∃ x, ∀ y, f x ≤ f y) : ∃ x, ∀ y, x ≠ y → f x < f y := by
