QuerySMT/cleanTests.lean
@@ -28,7 +28,40 @@ set_option auto.getHints.failOnParseError true
 -- set_option querySMT.filterHints false
 
 
--- Simple Algebraic Inequalities
+-- Simple Int Inequalities
+example (x y z : Int) : x < y → y < z → x < z := by
+  querySMT
+
+example (x y z : Int) : x < y → z < x → ¬z = y := by
+  querySMT
+
+example (w x y z : Int) : w <= x → x <= y → y <= z → z <= w → w = y := by
+  querySMT
+
+example (x y z : Int) : x <= y → y <= z → x = z → x = y ∧ y = z := by
+  querySMT
+
+example (x y z : Int) : x > y + z → x < y → z < 0 := by
+  querySMT
+
+-- Fails
+-- example (f : Int → Int) (h1 : ∀ x y : Int, x < y → f x < f y) : ∀ x y : Int, x ≠ y → f x ≠ f y := by
+--  querySMT
+
+example (f : Int → Int) (h1 : ∀ x y : Int, f x + f y ≤ x + y) : f 0 = 0 → ∀ x : Int, f x ≤ x := by
+  querySMT
+
+example (f : Int → Int) (h1 : ∀ x y : Int, f x = f y → x = y) : ∀ x y : Int, x ≠ y → f x ≠ f y := by
+  querySMT
+
+-- Fails
+-- example (f : Int → Int) (h1 : ∀ x y : Int, x < y → f x < f y) : ∀ x y : Int, f x = f y → x = y := by
+--  querySMT
+
+example (f g : Int → Int) (h1 : ∀ x : Int, f (g x) = x) : (∀ x y : Int, x ≠ y → g x ≠ g y) ∧ (∀ y : Int, ∃ x : Int, f x = y) := by
+  querySMT
+
+-- Simple Nat Inequalities
 
 -- Complex Algebraic Inequalities
 
